Added material on extended projective coordinates for Edwards curves, as well as a definition for the triple of parameters defining the particular curve edwards25519.
Also added a byte reversal function for machine words
with a few lemmas and a standard evaluation conversion
WORD_BYTEREVERSE_CONV, as usual extending the general
evaluation conversions like WORD_REDUCE_CONV to handle
it too.

New definitions:

        edwards25519
        edwards_excurve
        edwards_exprojadd
        edwards_exprojadd4
        edwards_exprojaddn
        exprojective
        word_bytereverse

and theorems:

        BIT_WORD_BYTEREVERSE
        EDWARDS_EXCURVE
        EDWARDS_EXPROJADD
        EDWARDS_EXPROJADD4
        EDWARDS_EXPROJADDN
        EDWARDS_EXPROJADD_DOUBLE
        EXPROJECTIVE_ALT
        WORD_BYTEREVERSE_BYTEREVERSE

Also fixed a few cases where the spelling wasn't as intended:

        EDWARD_NONSINGULAR_ALT    ->    EDWARDS_NONSINGULAR_ALT
        EDWARD_NONSINGULAR_25519  ->    EDWARDS_NONSINGULAR_25519
        EDWARD_NONSINGULAR_448    ->    EDWARDS_NONSINGULAR_448

EC/make.ml
@@ -22,12 +22,13 @@ loadt "EC/montgomery.ml";;
 loadt "EC/edwards.ml";;
 
 (* ------------------------------------------------------------------------- *)
-(* Projective, Jacobian and projective-without-y coordinates.                *)
+(* Projective, Jacobian, projective-without-y, extended projective coords.   *)
 (* ------------------------------------------------------------------------- *)
 
 loadt "EC/projective.ml";;
 loadt "EC/jacobian.ml";;
 loadt "EC/xzprojective.ml";;
+loadt "EC/exprojective.ml";;
 
 (* ------------------------------------------------------------------------- *)
 (* Some traditional formulas for evaluation in these coordinate systems.     *)
